AwsCryptographyPrimitives/runtimes/java/src/main/smithy-generated/software/amazon/cryptography/primitives/model/AES_CTR.java
@@ -1,0 +1,99 @@
+// Copyright Amazon.com Inc. or its affiliates. All Rights Reserved.
+// SPDX-License-Identifier: Apache-2.0
+// Do not modify this file. This file is machine generated, and any changes to it will be overwritten.
+package software.amazon.cryptography.primitives.model;
+
+import java.util.Objects;
+
+public class AES_CTR {
+  private final int keyLength;
+
+  private final int nonceLength;
+
+  protected AES_CTR(BuilderImpl builder) {
+    this.keyLength = builder.keyLength();
+    this.nonceLength = builder.nonceLength();
+  }
+
+  public int keyLength() {
+    return this.keyLength;
+  }
+
+  public int nonceLength() {
+    return this.nonceLength;
+  }
+
+  public Builder toBuilder() {
+    return new BuilderImpl(this);
+  }
+
+  public static Builder builder() {
+    return new BuilderImpl();
+  }
+
+  public interface Builder {
+    Builder keyLength(int keyLength);
+
+    int keyLength();
+
+    Builder nonceLength(int nonceLength);
+
+    int nonceLength();
+
+    AES_CTR build();
+  }
+
+  static class BuilderImpl implements Builder {
+    protected int keyLength;
+
+    protected int nonceLength;
+
+    protected BuilderImpl() {
+    }
+
+    protected BuilderImpl(AES_CTR model) {
+      this.keyLength = model.keyLength();
+      this.nonceLength = model.nonceLength();
+    }
+
+    public Builder keyLength(int keyLength) {
+      this.keyLength = keyLength;
+      return this;
+    }
+
+    public int keyLength() {
+      return this.keyLength;
+    }
+
+    public Builder nonceLength(int nonceLength) {
+      this.nonceLength = nonceLength;
+      return this;
+    }
+
+    public int nonceLength() {
+      return this.nonceLength;
+    }
+
+    public AES_CTR build() {
+      if (Objects.isNull(this.keyLength()))  {
+        throw new IllegalArgumentException("Missing value for required field `keyLength`");
+      }
+      if (Objects.nonNull(this.keyLength()) && this.keyLength() < 1) {
+        throw new IllegalArgumentException("`keyLength` must be greater than or equal to 1");
+      }
+      if (Objects.nonNull(this.keyLength()) && this.keyLength() > 32) {
+        throw new IllegalArgumentException("`keyLength` must be less than or equal to 32.");
+      }
+      if (Objects.isNull(this.nonceLength()))  {
+        throw new IllegalArgumentException("Missing value for required field `nonceLength`");
+      }
+      if (Objects.nonNull(this.nonceLength()) && this.nonceLength() < 0) {
+        throw new IllegalArgumentException("`nonceLength` must be greater than or equal to 0");
+      }
+      if (Objects.nonNull(this.nonceLength()) && this.nonceLength() > 255) {
+        throw new IllegalArgumentException("`nonceLength` must be less than or equal to 255.");
+      }
+      return new AES_CTR(this);
+    }
+  }
+}
