AwsCryptographyPrimitives/runtimes/net/Generated/AesKdfCtrInput.cs
@@ -3,39 +3,16 @@
 // Do not modify this file. This file is machine generated, and any changes to it will be overwritten.
 using System;
  using AWS.Cryptography.Primitives; namespace AWS.Cryptography.Primitives {
- public class HkdfInput {
- private AWS.Cryptography.Primitives.DigestAlgorithm _digestAlgorithm ;
- private System.IO.MemoryStream _salt ;
+ public class AesKdfCtrInput {
  private System.IO.MemoryStream _ikm ;
- private System.IO.MemoryStream _info ;
  private int? _expectedLength ;
- public AWS.Cryptography.Primitives.DigestAlgorithm DigestAlgorithm {
- get { return this._digestAlgorithm; }
- set { this._digestAlgorithm = value; }
-}
- public bool IsSetDigestAlgorithm () {
- return this._digestAlgorithm != null;
-}
- public System.IO.MemoryStream Salt {
- get { return this._salt; }
- set { this._salt = value; }
-}
- public bool IsSetSalt () {
- return this._salt != null;
-}
+ private System.IO.MemoryStream _nonce ;
  public System.IO.MemoryStream Ikm {
  get { return this._ikm; }
  set { this._ikm = value; }
 }
  public bool IsSetIkm () {
  return this._ikm != null;
-}
- public System.IO.MemoryStream Info {
- get { return this._info; }
- set { this._info = value; }
-}
- public bool IsSetInfo () {
- return this._info != null;
 }
  public int ExpectedLength {
  get { return this._expectedLength.GetValueOrDefault(); }
@@ -44,10 +21,15 @@ using System;
  public bool IsSetExpectedLength () {
  return this._expectedLength.HasValue;
 }
+ public System.IO.MemoryStream Nonce {
+ get { return this._nonce; }
+ set { this._nonce = value; }
+}
+ public bool IsSetNonce () {
+ return this._nonce != null;
+}
  public void Validate() {
- if (!IsSetDigestAlgorithm()) throw new System.ArgumentException("Missing value for required property 'DigestAlgorithm'");
  if (!IsSetIkm()) throw new System.ArgumentException("Missing value for required property 'Ikm'");
- if (!IsSetInfo()) throw new System.ArgumentException("Missing value for required property 'Info'");
  if (!IsSetExpectedLength()) throw new System.ArgumentException("Missing value for required property 'ExpectedLength'");
 
 }
