AwsCryptographyPrimitives/runtimes/net/Generated/ECDSAVerifyInput.cs
@@ -12,28 +12,28 @@ using System;
  get { return this._signatureAlgorithm; }
  set { this._signatureAlgorithm = value; }
 }
- internal bool IsSetSignatureAlgorithm () {
+ public bool IsSetSignatureAlgorithm () {
  return this._signatureAlgorithm != null;
 }
  public System.IO.MemoryStream VerificationKey {
  get { return this._verificationKey; }
  set { this._verificationKey = value; }
 }
- internal bool IsSetVerificationKey () {
+ public bool IsSetVerificationKey () {
  return this._verificationKey != null;
 }
  public System.IO.MemoryStream Message {
  get { return this._message; }
  set { this._message = value; }
 }
- internal bool IsSetMessage () {
+ public bool IsSetMessage () {
  return this._message != null;
 }
  public System.IO.MemoryStream Signature {
  get { return this._signature; }
  set { this._signature = value; }
 }
- internal bool IsSetSignature () {
+ public bool IsSetSignature () {
  return this._signature != null;
 }
  public void Validate() {
